add some solutions

chapter-3/ASM.thy
@@ -18,15 +18,19 @@ text{* Abbreviations are transparent: they are unfolded after
 parsing and folded back again before printing. Internally, they do not
 exist.*}
 
+text{* executes an instruction given a state *}
 fun exec1 :: "instr \<Rightarrow> state \<Rightarrow> stack \<Rightarrow> stack" 
   where "exec1 (LOADI n) _ stk = n # stk"
-  | "exec1 (LOAD x) s stk = s(x) # stk"
+  | "exec1 (LOAD x) state stk = state(x) # stk"
   | "exec1  ADD _ stk = (hd2 stk + hd stk) # tl2 stk"
 
+text{* executes a list of instructions given an initial state. (It's a fold) *}
 fun exec :: "instr list \<Rightarrow> state \<Rightarrow> stack \<Rightarrow> stack" 
   where "exec [] _ stk = stk" 
   | "exec (i#is) s stk = exec is s (exec1 i s stk)"
 
+text{* examples *}
+value "exec [LOAD ''x''] <''x'' := 2> [0]"
 value "exec [LOADI 5, LOAD ''y'', ADD] <''x'' := 42, ''y'' := 43> [50]"
 
 lemma exec_append[simp]:
@@ -37,12 +41,17 @@ done
 
 subsection "Compilation"
 
+text{* compiles an arithmetic expression to a list of instructions  *}
 fun comp :: "aexp \<Rightarrow> instr list" 
   where "comp (N n) = [LOADI n]" 
   | "comp (V x) = [LOAD x]" 
   | "comp (Plus e\<^sub>1 e\<^sub>2) = comp e\<^sub>1 @ comp e\<^sub>2 @ [ADD]"
 
+(* (x + 1) + z*)
 value "comp (Plus (Plus (V ''x'') (N 1)) (V ''z''))"
+
+(*let x = 2 and z = 4, then (x+1) + z = (2+1) + 4 = 7 *)
+value "exec (comp (Plus (Plus (V ''x'') (N 1)) (V ''z''))) <''x'':=2, ''z'':=4> []"
 
 theorem exec_comp: "exec (comp a) s stk = aval a s # stk"
 apply(induction a arbitrary: stk)
@@ -51,42 +60,107 @@ done
 
 text{* Exercises *}
 text{*
-Exercise 3.10. A stack underflow occurs when executing an ADD instruction on a stack of size
-               less than 2. In our semantics stack underflow lead to a term involving hd [],
-               which is not an error or exception (HOL does not have those concepts) but some
-               unspecified value. Modify theory ASM such that stack underflow is modelled by
-               None and normal execution by Some, i.e. the execution functions have return type
-               stack option. Modify all theorems and proofs accordingly.
+Exercise 3.10. 
+A stack underflow occurs when executing an ADD instruction on a stack of size
+less than 2. In our semantics stack underflow lead to a term involving hd [],
+which is not an error or exception (HOL does not have those concepts) but some
+unspecified value. Modify theory ASM such that stack underflow is modelled by
+None and normal execution by Some, i.e. the execution functions have return type
+stack option. Modify all theorems and proofs accordingly.
 *}
+fun exec1_opt :: "instr \<Rightarrow> state \<Rightarrow> stack \<Rightarrow> stack option" 
+  where "exec1_opt (LOADI n) _ stk = Some(n # stk)"
+  | "exec1_opt (LOAD x) state stk = Some(state(x) # stk)"
+  | "exec1_opt  ADD _ stk = (if length(stk) \<ge> 2 
+                             then Some( (hd2 stk + hd stk) # tl2 stk ) 
+                             else None)"
+
+text{* executes a list of instructions given an initial state. (It's a fold) *}
+fun exec_opt :: "instr list \<Rightarrow> state \<Rightarrow> stack \<Rightarrow> stack option" 
+  where "exec_opt [] _ stk = Some(stk)" 
+  | "exec_opt (i#is) s stk = 
+    (case (exec1_opt i s stk) of 
+       None       \<Rightarrow> None
+     | Some(stk') \<Rightarrow> exec_opt is s stk' )"
+
+text{* examples *}
+value "exec_opt [LOAD ''x''] <''x'' := 2> [0]"
+value "exec_opt [LOADI 5, LOAD ''y'', ADD] <''x'' := 42, ''y'' := 43> [50]"
+
+fun append_opt :: "('a list) option \<Rightarrow> ('a list) option \<Rightarrow> ('a list) option"
+  where "append_opt None _ = None"
+  | "append_opt (Some(l)) None = None"
+  | "append_opt (Some(l1)) (Some(l2)) = Some(l1@l2)"
+
+lemma exec_opt_append[simp]:
+  "(case (exec_opt is1 s stk) of
+      None       \<Rightarrow> None
+    | Some(stk') \<Rightarrow> exec_opt is2 s stk') = exec_opt (is1@is2) s stk"
+
+apply(induction is1 arbitrary: stk)
+apply(auto split: option.split)
+done
+
 
 text{*
-Exercise 3.11. This exercises is about a register machine and compiler for aexp.
-               The machine instructions are
-               datatype instr = LDI int reg | LD vname reg | ADD reg reg
-               where type reg is a synonym for nat. Instruction LDI i r loads i into
-               register r, LD x r loads the value of x into register r, and ADD r1 r2
-               adds register r2 to register r1.
-               Define the execution of an instruction given a state and a register state
-               (= function from registers to integers); the result is the new register state:
-               fun exec1 :: instr => state => (reg => int) => reg => int
-               Define the execution exec of a list of instructions as for the stack machine.
-               The compiler takes an arithmetic expression a and a register r and produces a
-               list of instructions whose execution places the value of a into r.
-               The registers > r should be used in a stack-like fashion for intermediate results,
-               the ones < r should be left alone. Define the compiler and prove it correct:
-               exec (comp a r) s rs r = aval a s
+Exercise 3.11. 
+This exercises is about a register machine and compiler for aexp.
+The machine instructions are 
+   datatype instr = LDI int reg | LD vname reg | ADD reg reg
+where type reg is a synonym for nat. Instruction LDI i r loads i into
+register r, LD x r loads the value of x into register r, and ADD r1 r2
+adds register r2 to register r1.
+Define the execution of an instruction given a state and a register state
+(= function from registers to integers); the result is the new register state:
+   fun exec1 :: instr => state => (reg => int) => reg => int
+Define the execution exec of a list of instructions as for the stack machine.
+The compiler takes an arithmetic expression a and a register r and produces a
+list of instructions whose execution places the value of a into r.
+The registers > r should be used in a stack-like fashion for intermediate results,
+the ones < r should be left alone. Define the compiler and prove it correct:
+   exec (comp a r) s rs r = aval a s
 *}
+
 type_synonym reg = "nat"
 type_synonym reg_state = "(reg \<Rightarrow> int)"
 
 datatype instr3
-  = LDI int reg
-  | LD vname reg
-  | ADD reg reg
+  = LDI int reg (* LDI n r loads n into register r *)
+  | LD vname reg (* LD x r loads the value of x into register r *)
+  | ADD reg reg (* ADD r1 r2 adds register r2 to register r1 *)
 
-fun exec1 :: "instr \<Rightarrow> state \<Rightarrow> reg_state \<Rightarrow> reg \<Rightarrow> int"
-  where "exec1 (LDI n reg) _ rstate r = "
-  | "exec1 (LD x r) state rstate r = " 
+fun exec1_instr3 :: "instr3 \<Rightarrow> state \<Rightarrow> reg_state \<Rightarrow> reg_state"
+  where "exec1_instr3 (LDI n reg) _ rstate = rstate(reg := n)"
+  | "exec1_instr3 (LD x r) state rstate = (let a = state(x) in rstate(r := a))"
+  | "exec1_instr3 (ADD r1 r2) state rstate = 
+      (let (r1val, r2val) = (rstate(r1), rstate(r2)) 
+       in rstate(r1 := r1val + r2val))"
+
+fun exec_instr3 :: "instr3 list \<Rightarrow> state \<Rightarrow> reg_state \<Rightarrow> reg_state" 
+  where "exec_instr3 [] _ rstate = rstate" 
+  | "exec_instr3 (i#is) state rstate = 
+      (let rstate' = exec1_instr3 i state rstate 
+       in exec_instr3 is state rstate')"
+
+lemma exec_instr3_append[simp]:
+  "exec_instr3 (is1@is2) s stk = exec_instr3 is2 s (exec_instr3 is1 s stk)"
+apply(induction is1 arbitrary: stk)
+apply (auto)
+done
+
+
+fun comp_instr3 :: "aexp \<Rightarrow> reg \<Rightarrow> instr3 list"
+  where "comp_instr3 (N n) r = [LDI n r]"
+  | "comp_instr3 (V x) r = [LD x r]"
+  | "comp_instr3 (Plus e1 e2) r 
+      = (comp_instr3 e1 r) @ (comp_instr3 e2 (r+1)) @ [ADD r (r+1)]"
+
+lemma exec_aval_equiv_instr3[simp]: 
+  "exec_instr3 (comp_instr3 a r) s rs r = aval a s"
+  apply(induction a arbitrary: r s rs)
+  apply(auto)
+  done (* this is failing *)
+
 text{*
 Exercise 3.12. This a variation on the previous exercise. Let the instruction set be
                datatype instr0 = LDI0 val | LD0 vname | MV0 reg | ADD0 reg
@@ -95,5 +169,11 @@ Exercise 3.12. This a variation on the previous exercise. Let the instruction se
                compiled code leaves the value of the expression in register 0. Prove that
                exec (comp a r) s rs 0 = aval a s
 *}
+
+datatype instr0
+  = LDI0 val
+  | LD0 vname
+  | MV0 reg
+  | ADD0 reg
 
 end
